Setlec/Verify/SimI.lean
@@ -671,7 +671,7 @@ theorem storedTyIdxM_eff (hs : ISOK mode env s₀) {n : Name} (x : Expr) :
       let ent? : Option IConstE ← modifyGet fun s => (s.ienv[n]?, s)
       match ent? with
       | some ent =>
-        if EStore.exprPtrBEq ent.tyE x then pure ent.ty
+        if Expr.exprPtrBEq ent.tyE x then pure ent.ty
         else internExprM x
       | none => internExprM x : CheckIM EIdx) from rfl] at hr
   simp only [Bind.bind, StateT.bind, modifyGet, MonadStateOf.modifyGet,
@@ -680,7 +680,7 @@ theorem storedTyIdxM_eff (hs : ISOK mode env s₀) {n : Name} (x : Expr) :
   | some ent =>
     rw [hl] at hr
     dsimp only at hr
-    by_cases hgate : EStore.exprPtrBEq ent.tyE x
+    by_cases hgate : Expr.exprPtrBEq ent.tyE x
     · rw [if_pos hgate] at hr
       have hEq : ent.tyE = x := by
         have : (ent.tyE == x) = true := hgate
@@ -704,7 +704,7 @@ theorem storedValIdxM_eff (hs : ISOK mode env s₀) {n : Name} (x : Expr) :
       let ent? : Option IConstE ← modifyGet fun s => (s.ienv[n]?, s)
       match ent? with
       | some ⟨_, _, some (vE, vi)⟩ =>
-        if EStore.exprPtrBEq vE x then pure vi
+        if Expr.exprPtrBEq vE x then pure vi
         else internExprM x
       | _ => internExprM x : CheckIM EIdx) from rfl] at hr
   simp only [Bind.bind, StateT.bind, modifyGet, MonadStateOf.modifyGet,
@@ -718,7 +718,7 @@ theorem storedValIdxM_eff (hs : ISOK mode env s₀) {n : Name} (x : Expr) :
       obtain ⟨vE, vi⟩ := p
       subst hval
       dsimp only at hr
-      by_cases hgate : EStore.exprPtrBEq vE x
+      by_cases hgate : Expr.exprPtrBEq vE x
       · rw [if_pos hgate] at hr
         have hEq : vE = x := by
           have : (vE == x) = true := hgate
